better support for 64-bit x86

examples/machine-code/hoare-triple/prog_x64Lib.sig
@@ -9,8 +9,13 @@ sig
     val x64_spec_byte_memory : string -> (thm * int * int option) *
                                          (thm * int * int option) option
 
-    val x64_tools            : decompiler_tools
-    val x64_tools_no_status  : decompiler_tools
+    val x64_spec_memory64    : string -> (thm * int * int option) *
+                                         (thm * int * int option) option
+
+    val x64_tools               : decompiler_tools
+    val x64_tools_no_status     : decompiler_tools
+    val x64_tools_64            : decompiler_tools
+    val x64_tools_64_no_status  : decompiler_tools
 
     val set_x64_exec_flag             : bool -> unit
     val set_x64_code_write_perm_flag  : bool -> unit
